tests/lean/run/dsimp_test.lean
@@ -4,29 +4,23 @@ def f : nat → nat
 
 open list tactic
 
-meta def check_expr (p : pexpr) (t : expr) : tactic unit :=
-do e ← to_expr p, guard (t = e)
-
-meta def check_target (p : pexpr) : tactic unit :=
-do t ← target, check_expr p t
-
 local attribute [-simp] map head
 
 example (a b c : nat) : head (map f [1, 2, 3]) = 20 :=
 begin
   dsimp [map],
-  check_target `(head [f 1, f 2, f 3] = 20),
+  guard_target head [f 1, f 2, f 3] = 20,
   dsimp [f],
-  check_target `(head [20 + 0, 20 + 1,  20 + 2] = 20),
+  guard_target head [20 + 0, 20 + 1,  20 + 2] = 20,
   dsimp [head],
-  check_target `(20 + 0 = 20),
+  guard_target 20 + 0 = 20,
   reflexivity
 end
 
 example (a b c : nat) : head (map f [1, 2, 3]) = 20 :=
 begin
   dsimp [map, f, head],
-  check_target `(20 + 0 = 20),
+  guard_target 20 + 0 = 20,
   reflexivity
 end
 
@@ -44,7 +38,7 @@ attribute [simp] gax
 example (a b c : nat) : g (f 1, f 2) = 41 :=
 begin
   dsimp,
-  check_target `(f 1 + f 2 = 41),
+  guard_target f 1 + f 2 = 41,
   dsimp [f],
   reflexivity
 end
@@ -52,16 +46,16 @@ end
 example (a b c : nat) : g (f 1, f 2) = 41 :=
 begin
   dsimp [f],
-  check_target `(20 + 0 + (20 + 1) = 41),
+  guard_target 20 + 0 + (20 + 1) = 41,
   reflexivity
 end
 
 example (a b c : nat) : g (f 1, f 2) = 41 :=
 begin
   dsimp [f] without gax,
-  check_target `(g (20 + 0, 20 + 1) = 41),
+  guard_target g (20 + 0, 20 + 1) = 41,
   dsimp [g],
-  check_target `(20 + 0 + (20 + 1) = 41),
+  guard_target 20 + 0 + (20 + 1) = 41,
   reflexivity
 end
 
@@ -70,15 +64,15 @@ local attribute [-simp] gax
 example (a b c : nat) : g (f 1, f 2) = 41 :=
 begin
   dsimp [f],
-  check_target `(g (20 + 0, 20 + 1) = 41),
+  guard_target g (20 + 0, 20 + 1) = 41,
   dsimp [gax],
-  check_target `(20 + 0 + (20 + 1) = 41),
+  guard_target 20 + 0 + (20 + 1) = 41,
   reflexivity
 end
 
 example (a b c : nat) : g (f 1, f 2) = 41 :=
 begin
   dsimp [f, gax],
-  check_target `(20 + 0 + (20 + 1) = 41),
+  guard_target 20 + 0 + (20 + 1) = 41,
   reflexivity
 end
