tests/lean/run/simp_attr_eqns.lean
@@ -1,11 +1,5 @@
 open nat tactic
 
-meta def check_expr (p : pexpr) (t : expr) : tactic unit :=
-do e ← to_expr p, guard (t = e)
-
-meta def check_target (p : pexpr) : tactic unit :=
-do t ← target, check_expr p t
-
 def g : nat → nat → nat :=
 λ x y, x * y
 
@@ -17,7 +11,7 @@ lemma ex0 (b a : nat) : b = f a → f (succ (succ a)) = g (g b 2) 2 :=
 begin
   intro h,
   simp [f],
-  check_target `(g (g (f a) 2) 2 = g (g b 2) 2),
+  guard_target g (g (f a) 2) 2 = g (g b 2) 2,
   subst b
 end
 
@@ -27,7 +21,7 @@ lemma ex1 (b a : nat) : b = f a → f (succ a) = g b 2 :=
 begin
   intro h,
   simp,
-  check_target `(g (f a) 2 = g b 2),
+  guard_target g (f a) 2 = g b 2,
   subst b
 end
 
@@ -35,7 +29,7 @@ lemma ex2 (b a : nat) : b = f a → f (succ (succ a)) = g (g b 2) 2 :=
 begin
   intro h,
   simp,
-  check_target `(g (g (f a) 2) 2 = g (g b 2) 2),
+  guard_target g (g (f a) 2) 2 = g (g b 2) 2,
   subst b
 end
 
@@ -44,7 +38,7 @@ local attribute [-simp] f
 lemma ex3 (b a : nat) : b = f a → f (succ a) = g b 2 :=
 begin
   intro h,
-  fail_if_success simp,
+  fail_if_success {simp},
   subst b,
   reflexivity
 end
@@ -57,6 +51,6 @@ lemma ex4 (b a : nat) : b = f a → f (succ a) = g b 2 :=
 begin
   intro h,
   simp with mysimp,
-  check_target `(g (f a) 2 = g b 2),
+  guard_target g (f a) 2 = g b 2,
   subst b
 end
