tests/lean/run/simp_partial_app.lean
@@ -1,16 +1,10 @@
 open tactic
 
-meta def check_expr (p : pexpr) (t : expr) : tactic unit :=
-do e ← to_expr p, guard (expr.alpha_eqv t e)
-
-meta def check_target (p : pexpr) : tactic unit :=
-do t ← target, check_expr p t
-
 example (a : list nat) : a = [1, 2] → a^.for nat.succ = [2, 3] :=
 begin
   intros,
   simp [list.for, flip],
-  check_target `(list.map nat.succ a = [2, 3]),
+  guard_target list.map nat.succ a = [2, 3],
   subst a,
   simp [list.map]
 end
